vale/code/arch/x64/X64.Vale.State.fsti
@@ -3,9 +3,9 @@ module X64.Vale.State
 
 open Prop_s
 open X64.Machine_s
-open X64.Vale
 open X64.Memory
-module F = FStar.FunctionalExtensionality
+module Regs = X64.Vale.Regs
+module Xmms = X64.Vale.Xmms
 
 noeq type state = {
   ok: bool;
@@ -16,30 +16,10 @@ noeq type state = {
   memTaint: memtaint;
 }
 
-let reg_to_int (r:reg) : int =
-  match r with
-  | Rax -> 0
-  | Rbx -> 1
-  | Rcx -> 2
-  | Rdx -> 3
-  | Rsi -> 4
-  | Rdi -> 5
-  | Rbp -> 6
-  | Rsp -> 7
-  | R8 -> 8
-  | R9 -> 9
-  | R10 -> 10
-  | R11 -> 11
-  | R12 -> 12
-  | R13 -> 13
-  | R14 -> 14
-  | R15 -> 15
-
-
 [@va_qattr]
-unfold let eval_reg (r:reg) (s:state) : nat64 = s.regs r
+unfold let eval_reg (r:reg) (s:state) : nat64 = Regs.sel r s.regs
 [@va_qattr]
-unfold let eval_xmm (x:xmm) (s:state) : Types_s.quad32 = s.xmms x
+unfold let eval_xmm (x:xmm) (s:state) : Types_s.quad32 = Xmms.sel x s.xmms
 [@va_qattr]
 unfold let eval_mem (ptr:int) (s:state) : GTot nat64 = load_mem64 ptr s.mem
 
@@ -64,14 +44,14 @@ let eval_operand (o:operand) (s:state) : GTot nat64 =
 
 [@va_qattr]
 let update_reg (r:reg) (v:nat64) (s:state) : state =
-  { s with regs = F.on_dom reg (fun r' -> if r = r' then v else s.regs r') }
+  {s with regs = Regs.upd r v s.regs}
 
 [@va_qattr]
 let update_xmm (x:xmm) (v:Types_s.quad32) (s:state) : state =
-  { s with xmms = F.on_dom xmm (fun x' -> if x = x' then v else s.xmms x') }
+  {s with xmms = Xmms.upd x v s.xmms}
 
 [@va_qattr]
-let update_mem (ptr:int) (v:nat64) (s:state) : GTot state = { s with mem = store_mem64 ptr v s.mem }
+let update_mem (ptr:int) (v:nat64) (s:state) : GTot state = {s with mem = store_mem64 ptr v s.mem}
 
 [@va_qattr]
 let update_operand (o:operand) (v:nat64) (sM:state) : GTot state =
@@ -89,6 +69,10 @@ let valid_operand (o:operand) (s:state) : prop0 =
   | OConst n -> 0 <= n /\ n < pow2_64
   | OReg r -> True
   | OMem m -> valid_maddr m s
+
+[@va_qattr]
+let state_eta (s:state) : state =
+  {s with regs = Regs.eta s.regs; xmms = Xmms.eta s.xmms}
 
 [@va_qattr]
 let state_eq (s0:state) (s1:state) : prop0 =
